can get topic-name

src/utils.fst
@@ -2,7 +2,20 @@ module Utils
 
 open FStar.HyperStack.ST
 module U8 = FStar.UInt8
+module U32 = FStar.UInt32
+module B = LowStar.Buffer
+module HS = FStar.HyperStack
+
+let zero_terminated_buffer_u8 (h: HS.mem) (b: B.buffer U8.t) =
+  let s = B.as_seq h b in
+  B.length b > 0 /\
+  B.length b <= FStar.UInt.max_int 32 /\
+  U8.v (Seq.index s (B.length b - 1)) = 0
 
 assume val print_hex (i:U8.t): Stack unit
   (requires (fun h -> true))
+  (ensures (fun h0 ret h1 -> true))
+
+assume val buffer_uint8_to_c_string: u8_buffer: B.buffer U8.t -> Stack C.String.t
+  (requires (fun h -> B.live h u8_buffer /\ zero_terminated_buffer_u8 h u8_buffer))
   (ensures (fun h0 ret h1 -> true))
